Added Arden's Rule
- Changed definitions in Regex.Basic
- Updated affected files (Regex2NFA)

lean4/Automaton/Language/Basic.lean
@@ -7,3 +7,7 @@ def word : Type _ := List Sigma
 
 @[reducible]
 def Lang : Type _ := Set (word Sigma)
+
+def power {Sigma : _ } (l : word Sigma) : Nat → word Sigma
+  | 0  => []
+  | n+1  => l ++ power l n
