lean4/Automaton/Regex/Regex2NFA.lean
@@ -9,11 +9,11 @@ namespace ToNFA
 
 open NFA Regex
 
-variable {σ : Type _} {σs : Finset σ} [DecidableEq σ]
+variable {σ : Type _} {σs : Finset σ} [DecidableEq σ] {a : Regex σs}
 
 
 def regex2NFA : Regex σs → NFA σs
-  | Regex.zero => Zero.zeroNfa
+  | Regex.zero => Zero.zero_nfa
   | Regex.epsilon => Empty.empty
   | Regex.char a => Char.char a
   | Regex.plus a b => Plus.plus_nfa (regex2NFA a) (regex2NFA b)
@@ -21,9 +21,9 @@ def regex2NFA : Regex σs → NFA σs
   | Regex.star a => Plus.plus_nfa (Star.star_nfa (regex2NFA a)) (Empty.empty)
 
 
-theorem star_to_regex (s₁ : w ∈ nfaLang (regex2NFA a) → w ∈ RegexLan σs a)
-  (s₂ : ∀ w', w'.length < w.length → w' ∈ nfaLang (regex2NFA a) → w' ∈ RegexLan σs a)
-  (h : w ∈ nfaLang (regex2NFA (Regex.star a))) : w ∈ RegexLan σs (Regex.star a) := by
+theorem star_to_regex (s₁ : w ∈ nfaLang (regex2NFA a) → w ∈ regexLan a)
+  (s₂ : ∀ w', w'.length < w.length → w' ∈ nfaLang (regex2NFA a) → w' ∈ regexLan a)
+  (h : w ∈ nfaLang (regex2NFA (Regex.star a))) : w ∈ regexLan (Regex.star a) := by
   simp only [nfaLang,Set.mem_def,regex2NFA] at h
   rw [Plus.accepts_iff,Star.accepts_iff] at h
   apply Or.elim h
@@ -32,7 +32,7 @@ theorem star_to_regex (s₁ : w ∈ nfaLang (regex2NFA a) → w ∈ RegexLan σs
     · intro h
       have : w = w ++ [] := by simp
       rw [this]
-      simp only [RegexLan]
+      simp only [regexLan]
       apply starLang.extend
       · exact s₁  h
       · apply starLang.empty
@@ -65,14 +65,14 @@ theorem star_to_regex (s₁ : w ∈ nfaLang (regex2NFA a) → w ∈ RegexLan σs
   · intro em
     rw [Empty.accepts_iff] at em
     rw [em]
-    simp only [RegexLan]
+    simp only [regexLan]
     apply starLang.empty
 termination_by star_to_regex => w.length
 
-theorem regex_to_star (s₁ : w ∈ RegexLan σs a → w ∈ nfaLang (regex2NFA a))
-  (s₂ : ∀ w', w'.length < w.length → w' ∈ RegexLan σs a → w' ∈ nfaLang (regex2NFA a))
-  (h : w ∈ RegexLan σs (Regex.star a)) : w ∈ nfaLang (regex2NFA (Regex.star a)) := by
-  simp only [RegexLan] at h
+theorem regex_to_star (s₁ : w ∈ regexLan a → w ∈ nfaLang (regex2NFA a))
+  (s₂ : ∀ w', w'.length < w.length → w' ∈ regexLan a → w' ∈ nfaLang (regex2NFA a))
+  (h : w ∈ regexLan (Regex.star a)) : w ∈ nfaLang (regex2NFA (Regex.star a)) := by
+  simp only [regexLan] at h
   rw [mem_starLang_iff] at h
   simp only [nfaLang,regex2NFA,Set.mem_def,Plus.accepts_iff]
   apply Or.elim h
@@ -104,8 +104,8 @@ theorem regex_to_star (s₁ : w ∈ RegexLan σs a → w ∈ nfaLang (regex2NFA 
                exists a'
                exists b::bs
                use h.1, h.2.1, s₂ a' lt₂ h.2.2.1
-               have bin : b::bs ∈ RegexLan σs (Regex.star a) := by simp only [RegexLan]; exact h.2.2.2
-               have fa : ∀ w', w'.length < (b::bs).length → RegexLan σs a w' → nfa_accepts (regex2NFA a) w' := by
+               have bin : b::bs ∈ regexLan (Regex.star a) := by simp only [regexLan]; exact h.2.2.2
+               have fa : ∀ w', w'.length < (b::bs).length → regexLan a w' → nfa_accepts (regex2NFA a) w' := by
                 intro w' lt r
                 apply s₂ _ (Nat.lt_trans lt lt₁) r
                have := regex_to_star (s₂ _ lt₁) fa bin
@@ -119,15 +119,15 @@ theorem regex_to_star (s₁ : w ∈ RegexLan σs a → w ∈ nfaLang (regex2NFA 
                  contradiction
 termination_by regex_to_star => w.length
 
-theorem append_to_regex (s₁: w ∈ nfaLang (regex2NFA a) → w ∈ RegexLan σs a)
-  (s₂: w ∈ nfaLang (regex2NFA b) → w ∈ RegexLan σs b)
+theorem append_to_regex (s₁: w ∈ nfaLang (regex2NFA a) → w ∈ regexLan a)
+  (s₂: w ∈ nfaLang (regex2NFA b) → w ∈ regexLan b)
   (h: w ∈ nfaLang (regex2NFA (Regex.append a b)))
-  (fa₁: ∀ (w' : List { x // x ∈ σs }), List.length w' < List.length w → w' ∈ nfaLang (regex2NFA a) → w' ∈ RegexLan σs a)
-  (fa₂: ∀ (w' : List { x // x ∈ σs }), List.length w' < List.length w → w' ∈ nfaLang (regex2NFA b) → w' ∈ RegexLan σs b) : w ∈ RegexLan σs (Regex.append a b) := by
+  (fa₁: ∀ (w' : List { x // x ∈ σs }), List.length w' < List.length w → w' ∈ nfaLang (regex2NFA a) → w' ∈ regexLan a)
+  (fa₂: ∀ (w' : List { x // x ∈ σs }), List.length w' < List.length w → w' ∈ nfaLang (regex2NFA b) → w' ∈ regexLan b) : w ∈ regexLan (Regex.append a b) := by
   simp only [regex2NFA,nfaLang,Append.accepts_iff,Set.mem_def] at h
   simp only [nfaLang,Set.mem_def] at s₁
   simp only [nfaLang,Set.mem_def] at s₂
-  simp only [RegexLan,Set.mem_def,setOf]
+  simp only [regexLan,Set.mem_def,setOf]
   apply Exists.elim h
   intro a ex
   apply Exists.elim ex
@@ -172,12 +172,12 @@ theorem append_to_regex (s₁: w ∈ nfaLang (regex2NFA a) → w ∈ RegexLan σ
                                    use fa₂ _ lt₂ h.2.1
                                    rw [←h.2.2]
 
-theorem regex_to_append (s₁: w ∈ RegexLan σs a → w ∈ nfaLang (regex2NFA a) )
-  (s₂: w ∈ RegexLan σs b → w ∈ nfaLang (regex2NFA b))
-  (h: w ∈ RegexLan σs (Regex.append a b))
-  (fa₁: ∀ (w' : List { x // x ∈ σs }), List.length w' < List.length w → w' ∈ RegexLan σs a → w' ∈ nfaLang (regex2NFA a))
-  (fa₂: ∀ (w' : List { x // x ∈ σs }), List.length w' < List.length w → w' ∈ RegexLan σs b → w' ∈ nfaLang (regex2NFA b)) : w ∈ nfaLang (regex2NFA (Regex.append a b)) := by
-  simp only [RegexLan,Set.mem_def,setOf] at h
+theorem regex_to_append (s₁: w ∈ regexLan a → w ∈ nfaLang (regex2NFA a) )
+  (s₂: w ∈ regexLan b → w ∈ nfaLang (regex2NFA b))
+  (h: w ∈ regexLan (Regex.append a b))
+  (fa₁: ∀ (w' : List { x // x ∈ σs }), List.length w' < List.length w → w' ∈ regexLan a → w' ∈ nfaLang (regex2NFA a))
+  (fa₂: ∀ (w' : List { x // x ∈ σs }), List.length w' < List.length w → w' ∈ regexLan b → w' ∈ nfaLang (regex2NFA b)) : w ∈ nfaLang (regex2NFA (Regex.append a b)) := by
+  simp only [regexLan,Set.mem_def,setOf] at h
   simp only [regex2NFA,nfaLang,Set.mem_def,Append.accepts_iff]
   apply Exists.elim h
   intro a ex
@@ -216,14 +216,14 @@ theorem regex_to_append (s₁: w ∈ RegexLan σs a → w ∈ nfaLang (regex2NFA
                                    use fa₂ _ lt₂ h.2.1
                                    rw [←h.2.2]
 
-theorem nfa2regex : w ∈ nfaLang (regex2NFA r) → w ∈ RegexLan σs r := by
+theorem nfa2regex {r : Regex σs} : w ∈ nfaLang (regex2NFA r) → w ∈ regexLan r := by
   intro h
   induction r with
-  | zero => simp only [regex2NFA,nfaLang,Zero.accepts_iff] at h; simp only [RegexLan]; apply h
-  | epsilon => simp only [regex2NFA,nfaLang,Empty.accepts_iff] at h; simp only [RegexLan]; apply h
-  | char a => simp only [regex2NFA,nfaLang,Char.accepts_iff] at h; simp only [RegexLan]; apply h
+  | zero => simp only [regex2NFA,nfaLang,Zero.accepts_iff] at h; simp only [regexLan]; apply h
+  | epsilon => simp only [regex2NFA,nfaLang,Empty.accepts_iff] at h; simp only [regexLan]; apply h
+  | char a => simp only [regex2NFA,nfaLang,Char.accepts_iff] at h; simp only [regexLan]; apply h
   | plus a b s₁ s₂ => simp only [regex2NFA,nfaLang,regex2NFA,Plus.accepts_iff,Set.mem_def] at h
-                      simp only [RegexLan,Set.mem_union]
+                      simp only [regexLan,Set.mem_union]
                       apply Or.elim h
                       · intro h
                         apply Or.inl
@@ -231,27 +231,27 @@ theorem nfa2regex : w ∈ nfaLang (regex2NFA r) → w ∈ RegexLan σs r := by
                       intro h
                       apply Or.inr
                       apply s₂ h
-  | append a b s₁ s₂ => have fa₁ : ∀ w', List.length w' < List.length w → w' ∈ nfaLang (regex2NFA a) → w' ∈ RegexLan σs a := by
+  | append a b s₁ s₂ => have fa₁ : ∀ w', List.length w' < List.length w → w' ∈ nfaLang (regex2NFA a) → w' ∈ regexLan a := by
                           intro w' _ w'in
                           exact nfa2regex w'in
-                        have fa₂ : ∀ w', List.length w' < List.length w → w' ∈ nfaLang (regex2NFA b) → w' ∈ RegexLan σs b := by
+                        have fa₂ : ∀ w', List.length w' < List.length w → w' ∈ nfaLang (regex2NFA b) → w' ∈ regexLan b := by
                           intro w' _ w'in
                           exact nfa2regex w'in
                         apply append_to_regex s₁ s₂ h fa₁ fa₂
-  | star a s => have fa : ∀ w', List.length w' < List.length w → w' ∈ nfaLang (regex2NFA a) → w' ∈ RegexLan σs a := by
+  | star a s => have fa : ∀ w', List.length w' < List.length w → w' ∈ nfaLang (regex2NFA a) → w' ∈ regexLan a := by
                   intro w' _ w'in
                   exact nfa2regex w'in
                 apply star_to_regex s fa h
 termination_by nfa2regex => w.length
 
-theorem regex2nfa : w ∈ RegexLan σs r → w ∈ nfaLang (regex2NFA r) := by
+theorem regex2nfa {r : Regex σs} : w ∈ regexLan r → w ∈ nfaLang (regex2NFA r) := by
   intro h
   induction r with
-  | zero => simp only [RegexLan] at h; simp only [regex2NFA,nfaLang,Zero.accepts_iff,Set.mem_def]; apply h
+  | zero => simp only [regexLan] at h; simp only [regex2NFA,nfaLang,Zero.accepts_iff,Set.mem_def]; apply h
   | epsilon => simp only [regex2NFA,nfaLang,Empty.accepts_iff]; apply h
   | char a => simp only [regex2NFA,nfaLang,Char.accepts_iff]; apply h
   | plus a b s₁ s₂ => simp only [regex2NFA,nfaLang,regex2NFA,Plus.accepts_iff,Set.mem_def]
-                      simp only [RegexLan,Set.mem_union] at h
+                      simp only [regexLan,Set.mem_union] at h
                       apply Or.elim h
                       · intro h
                         apply Or.inl
@@ -259,20 +259,20 @@ theorem regex2nfa : w ∈ RegexLan σs r → w ∈ nfaLang (regex2NFA r) := by
                       intro h
                       apply Or.inr
                       apply s₂ h
-  | append a b s₁ s₂ => have fa₁ : ∀ w', List.length w' < List.length w → w' ∈ RegexLan σs a → w' ∈ nfaLang (regex2NFA a):= by
+  | append a b s₁ s₂ => have fa₁ : ∀ w', List.length w' < List.length w → w' ∈ regexLan a → w' ∈ nfaLang (regex2NFA a):= by
                           intro w' _ w'in
                           exact regex2nfa w'in
-                        have fa₂ : ∀ w', List.length w' < List.length w →  w' ∈ RegexLan σs b → w' ∈ nfaLang (regex2NFA b) := by
+                        have fa₂ : ∀ w', List.length w' < List.length w →  w' ∈ regexLan b → w' ∈ nfaLang (regex2NFA b) := by
                           intro w' _ w'in
                           exact regex2nfa w'in
                         exact regex_to_append s₁ s₂ h fa₁ fa₂
-  | star a s => have fa : ∀ w', List.length w' < List.length w → w' ∈ RegexLan σs a → w' ∈ nfaLang (regex2NFA a) := by
+  | star a s => have fa : ∀ w', List.length w' < List.length w → w' ∈ regexLan a → w' ∈ nfaLang (regex2NFA a) := by
                   intro w' _ w'in
                   exact regex2nfa w'in
                 apply regex_to_star s fa h
 termination_by regex2nfa => w.length
 
-theorem regex2NFA_eq_regex : nfaLang (regex2NFA r) = RegexLan σs r := by
+theorem regex2NFA_eq_regex : nfaLang (regex2NFA a) = regexLan a := by
   rw [Set.ext_iff]
   intro x
   apply Iff.intro
