lean4/Automaton/Regex/Zero.lean
@@ -8,12 +8,12 @@ namespace Zero
 
 variable {σ : Type _} (q₁ q₂ : Type _) {σs : Finset σ}  [DecidableEq q₁] [DecidableEq q₂] [DecidableEq σ]
 
-def zeroNfa : NFA σs := {q := Nat, qs := {}, q₀ := {}, fs := {}, δ := fun _ _ => {}}
+def zero_nfa : NFA σs := {q := Nat, qs := {}, q₀ := {}, fs := {}, δ := fun _ _ => {}}
 
-theorem accepts_iff (w : word σs) : nfa_accepts zeroNfa w ↔ False := by
+theorem accepts_iff (w : word σs) : nfa_accepts zero_nfa w ↔ False := by
   apply Iff.intro
   · intro na
-    simp only [zeroNfa,nfa_accepts,Finset.Nonempty] at na
+    simp only [zero_nfa,nfa_accepts,Finset.Nonempty] at na
     apply Exists.elim na
     intro x xin
     rw [Finset.mem_inter] at xin
